R1cs.v
@@ -11,7 +11,6 @@ Import Z.
 Require Import Coq.Init.Nat.
 Require Import Coq.Vectors.VectorDef.
 Require Import Coq.Vectors.Fin.
-Require Import Coq.micromega.Lia.
 
 (**
    1. Use a state monad to compile equations to R1CS
@@ -30,168 +29,194 @@ Require Import Coq.micromega.Lia.
  *)
 Module R1CS(PF: GaloisField).
   Import PF.
-  
+  Import VectorNotations.
+  Set Printing Implicit.
   Definition Vfp := Vector.t Fp.
   
-  Inductive term: nat -> nat -> Set :=
-  | input: forall (n: nat), term (S n) 0
-  | var: forall (n: nat), term 0 (S n)
-  | one: term 0 0.
+  Inductive term: nat -> nat -> nat -> Set :=
+  | input: forall (n: nat), term (S n) 0 0
+  | output: forall (n: nat), term 0 (S n) 0
+  | var: forall (n: nat), term 0 0 (S n)
+  | one: term 0 0 0.
 
-  Inductive additions: nat -> nat -> Type :=
-  | ahead: forall m n, Fp * term m n -> additions m n
-  | atail: forall a b c d,
-      Fp * term a b ->
-      additions c d ->
-      additions (max a c) (max b d).
+  Inductive additions: nat -> nat -> nat -> Type :=
+  | ahead: forall i o v, Fp * term i o v -> additions i o v
+  | atail: forall i o v i' o' v',
+      Fp * term i o v ->
+      additions i' o' v' ->
+      additions (max i i') (max o o') (max v v').
   
-  Definition max3(a b c: nat) := max a (max b c).
-  Hint Unfold max3: core.
+  Inductive constraint: nat -> nat -> nat -> Type :=
+  | lc: forall i o v i' o' v' i'' o'' v''
+      (A: additions i o v)
+      (B: additions i' o' v')
+      (C: additions i'' o'' v''),
+      constraint (max i (max i' i'')) (max o (max o' o'')) (max v (max v' v'')).
 
-  Inductive constraint: nat -> nat -> Type :=
-  | lc: forall a b c d e f
-      (A: additions a b)
-      (B: additions c d)
-      (C: additions e f),
-      constraint (max3 a c e) (max3 b d f).
+  Inductive r1cs: nat -> nat -> nat -> nat -> Type :=
+  | rnil: r1cs 0 0 0 0
+  | rcons: forall n i o v i' o' v',
+      constraint i o v ->
+      r1cs n i' o' v' ->
+      r1cs (S n) (max i i') (max o o') (max v v').
 
-  Inductive r1cs: nat -> nat -> nat -> Type :=
-  | rhead: forall m n,
-      constraint m n ->
-      r1cs 1 m n
-  | rtail: forall a b c d n,
-      constraint a b ->
-      r1cs n c d ->
-      r1cs (S n) (max a c) (max b d).
+  
+  Arguments additions {i} {o} {v}.
+  Arguments ahead {i} {o} {v}.
+  Arguments atail {i} {o} {v} {i'} {o'} {v'}.
+  Arguments constraint {i} {o} {v}.
+  Arguments lc {i} {o} {v} {i'} {o'} {v'} {i''} {o''} {v''}.
+  Arguments rcons {n} {i} {o} {v} {i'} {o'} {v'}.
+  Arguments r1cs {n} {i} {o} {v}.
 
-  Arguments additions {m} {n}.
-  Arguments ahead {m} {n}.
-  Arguments atail {a} {b} {c} {d}.
-  Arguments constraint {a} {b}.
-  Arguments lc {a} {b} {c} {d} {e} {f}.
-  Arguments rhead {m} {n}.
-  Arguments rtail {a} {b} {c} {d} {n}.
-  Arguments r1cs {a} {b} {c}.
+  Definition r1cs_singleton{i o v}(c: @constraint i o v) :=
+    rcons c rnil.
 
   (** syntax *)
   Declare Custom Entry r1cs.
-  Notation "<[ e ]>" := e (e custom r1cs at level 90).
-  Notation "z 'i[' n ']'" :=
-    (to_p z, input n%nat)
-      (in custom r1cs at level 2,
-          n constr at level 0,
-          z constr at level 0).
-  Notation "z 'v[' n ']'" :=
-    (to_p z, var n%nat)
-      (in custom r1cs at level 2,
-          n constr at level 0,
-          z constr at level 0).
-  Notation "z 1" :=
-    (to_p z, one)
-      (in custom r1cs at level 2,
-          z constr at level 0).
-  Notation "{ x }" := x (in custom r1cs, x constr).
-  Notation "( a )" :=
-    (ahead a) (in custom r1cs at level 4, a custom r1cs at level 2).
-
-  Notation "( a1 + .. + a2 + a3 )" :=
-    (atail a1 .. (atail a2 (ahead a3)) ..)
-      (in custom r1cs at level 4,
-          a1 custom r1cs at level 2,
-          a2 custom r1cs at level 2,
-          a3 custom r1cs at level 2).
-
-  Notation "# a * b == c" :=
-    (lc a b c)
-      (in custom r1cs at level 90,
-          a custom r1cs at level 4,
-          b custom r1cs at level 4,
-          c custom r1cs at level 4,
+  
+  Notation "<[ x ; .. ; y ]>" :=
+    (rcons x .. (rcons y rnil) ..)
+      (at level 1,
+          x custom r1cs at level 2,
+          y custom r1cs at level 2,
           left associativity).
 
-  Coercion rhead: constraint >-> r1cs.
+  Notation "'{' a '*' b '==' c '}'" :=
+    (lc a b c)
+      (in custom r1cs at level 2,
+          a custom r1cs at level 3,
+          b custom r1cs at level 3,
+          c custom r1cs at level 3,
+          left associativity).
 
-  Lemma le_lt_Sn_m: forall n m, S n <= m -> n < m. lia. Qed.
+  Notation "( a )" :=
+    (ahead a) (in custom r1cs at level 3, a custom r1cs at level 4).
   
-  Set Printing Implicit.
-  Fixpoint eval_additions{i v i' v'}
-           (adds: @additions i v)
+  Notation "( a1 + .. + a2 + a3 )" :=
+    (atail a1 .. (atail a2 (ahead a3)) ..)
+      (in custom r1cs at level 3,
+          a1 custom r1cs at level 4,
+          a2 custom r1cs at level 4,
+          a3 custom r1cs at level 4).
+
+  Notation "z 'i[' n ']'" :=
+    (to_p z, input n%nat)
+      (in custom r1cs at level 4,
+          n constr,
+          z constr).
+  
+  Notation "z 'o[' n ']'" :=
+    (to_p z, output n%nat)
+      (in custom r1cs at level 4,
+          n constr,
+          z constr).
+  
+  Notation "z 'v[' n ']'" :=
+    (to_p z, var n%nat)
+      (in custom r1cs at level 4,
+          n constr,
+          z constr).
+  
+  Notation "[ z ]" :=
+    (to_p z, one)
+      (in custom r1cs at level 4,
+          z constr at level 0).
+
+  Coercion r1cs_singleton: constraint >-> r1cs.
+  Eval cbn in <[ { (3o[0] + 3i[1]) * (3i[0] + 2v[2]) == ([1]) };{ (3o[0] + 3i[1]) * (3i[0] + 2v[2]) == ([1]) }  ]>.   
+
+  Fixpoint eval_additions{i o v i' o' v'}
+           (adds: @additions i o v)
            (inputs: Vfp i')
-           (vars: Vfp v'): i <= i' -> v <= v' -> Fp.
+           (outputs: Vfp o')
+           (vars: Vfp v'): i <= i' -> o <= o' -> v <= v' -> Fp.
     invert adds; intros.
-    - invert H; invert H3.
-      + apply le_lt_Sn_m in H0; clear H1.
-        exact (pkmul H2 (Vector.nth inputs (Fin.of_nat_lt H0))). (** Fp * Input term *)
-      + apply le_lt_Sn_m in H1; clear H0.
-        exact (pkmul H2 (Vector.nth vars (Fin.of_nat_lt H1))).   (** Fp * Var term *)
-      + exact H2. (** Fp * 1 (One) term *)
-    - specialize (eval_additions _ _ _ _ H0 inputs vars) as Hprev.
+    - invert H; invert H4.
+      + apply le_lt_Sn_m in H0; clear H1 H2.
+        exact (pkmul H3 (Vector.nth inputs (Fin.of_nat_lt H0))).  (** Fp * Input term *)
+      + apply le_lt_Sn_m in H1; clear H0 H2.
+        exact (pkmul H3 (Vector.nth outputs (Fin.of_nat_lt H1))). (** Fp * Output term *)
+      + apply le_lt_Sn_m in H2; clear H0 H1.
+        exact (pkmul H3 (Vector.nth vars (Fin.of_nat_lt H2))).    (** Fp * Var term *)
+      + exact H3. (** Fp * 1 (One) term *)
+    - specialize (eval_additions _ _ _ _ _ _ H0 inputs outputs vars) as Hprev.
       pose proof (Nat.max_lub_r _ _ _ H1).
       pose proof (Nat.max_lub_r _ _ _ H2).
+      pose proof (Nat.max_lub_r _ _ _ H3).
       pose proof (Nat.max_lub_l _ _ _ H1).
       pose proof (Nat.max_lub_l _ _ _ H2).
-      clear H1 H2.
+      pose proof (Nat.max_lub_l _ _ _ H3).
+      clear H1 H2 H3.
       invert H; invert H2.
-      + apply le_lt_Sn_m in H5; clear H6.
-        exact (pkplus (Hprev H3 H4) (pkmul H1 (Vector.nth inputs (Fin.of_nat_lt H5)))).
-      + apply le_lt_Sn_m in H6; clear H5.
-        exact (pkplus (Hprev H3 H4) (pkmul H1 (Vector.nth vars (Fin.of_nat_lt H6)))).
-      + exact (pkplus (Hprev H3 H4) H1).
+      + apply le_lt_Sn_m in H7; clear H8 H9.
+        exact (pkplus (Hprev H4 H5 H6) (pkmul H1 (Vector.nth inputs (Fin.of_nat_lt H7)))).
+      + apply le_lt_Sn_m in H8; clear H7 H9.
+        exact (pkplus (Hprev H4 H5 H6) (pkmul H1 (Vector.nth outputs (Fin.of_nat_lt H8)))).
+      + apply le_lt_Sn_m in H9; clear H7 H8.
+        exact (pkplus (Hprev H4 H5 H6) (pkmul H1 (Vector.nth vars (Fin.of_nat_lt H9)))).
+      + exact (pkplus (Hprev H4 H5 H6) H1).
   Defined.
 
-  Print eval_additions.
-  Fixpoint eval_constraint{i v i' v'}
-           (ctr: @constraint i v)
+  Fixpoint eval_constraint{i o v i' o' v'}
+           (ctr: @constraint i o v)
            (inputs: Vfp i')
-           (vars: Vfp v') : i <= i' -> v <= v' -> Fp.
+           (outputs: Vfp o')
+           (vars: Vfp v') : i <= i' -> o <= o' -> v <= v' -> Fp.
     invert ctr.
     intros.
-    unfold max3 in *.
     pose proof (Nat.max_lub_r _ _ _ H).
     pose proof (Nat.max_lub_r _ _ _ H0).
+    pose proof (Nat.max_lub_r _ _ _ H1).
     pose proof (Nat.max_lub_l _ _ _ H).
     pose proof (Nat.max_lub_l _ _ _ H0).
-    pose proof (Nat.max_lub_r _ _ _ H1).
-    pose proof (Nat.max_lub_r _ _ _ H2).
     pose proof (Nat.max_lub_l _ _ _ H1).
+    pose proof (Nat.max_lub_r _ _ _ H2).
+    pose proof (Nat.max_lub_r _ _ _ H3).
+    pose proof (Nat.max_lub_r _ _ _ H4).
     pose proof (Nat.max_lub_l _ _ _ H2).
-    clear H H0 H1 H2.
-    pose proof (eval_additions A inputs vars H3 H4) as SumA.
-    pose proof (eval_additions B inputs vars H7 H8) as SumB.
-    pose proof (eval_additions C inputs vars H5 H6) as SumC.
-    exact (pksub (pkmul SumA SumB) SumC). (** A*B - C *)
+    pose proof (Nat.max_lub_l _ _ _ H3).
+    pose proof (Nat.max_lub_l _ _ _ H4).    
+    clear H H0 H1 H2 H3 H4.
+    pose proof (eval_additions A inputs outputs vars H5 H6 H7) as SumA.
+    pose proof (eval_additions B inputs outputs vars H11 H12 H13) as SumB.
+    pose proof (eval_additions C inputs outputs vars H8 H9 H10) as SumC.
+    exact (pksub (pkmul SumA SumB) SumC). (** A * B - C *)
   Defined.
 
-  Fixpoint eval_fix{n i v i' v'}
-           (r: @r1cs n i v)
+  Import VectorNotations.
+  Fixpoint eval_fix{n i o v i' o' v'}
+           (r: @r1cs n i o v)
            (inputs: Vfp i')
-           (vars: Vfp v'): i <= i' -> v <= v' -> Vfp n.
+           (outputs: Vfp o')
+           (vars: Vfp v'): i <= i' -> o <= o' -> v <= v' -> Vfp n.
   Proof.
     intros.
     invert r.
-    - pose proof (eval_constraint H1 inputs vars H H0) as CtrEval.
-      exact (Vector.cons Fp CtrEval 0 (Vector.nil Fp)).
+    - exact [].
     - pose proof (Nat.max_lub_r _ _ _ H).
       pose proof (Nat.max_lub_l _ _ _ H).
       pose proof (Nat.max_lub_r _ _ _ H0).
-      pose proof (Nat.max_lub_l _ _ _ H0).         
-      pose proof (eval_fix _ _ _ _ _ H2 inputs vars H3 H5) as Hprev.
-      pose proof (eval_constraint H1 inputs vars H4 H6) as CtrEval.
-      exact (Vector.cons Fp CtrEval n0 Hprev).
+      pose proof (Nat.max_lub_l _ _ _ H0).
+      pose proof (Nat.max_lub_r _ _ _ H1).
+      pose proof (Nat.max_lub_l _ _ _ H1).      
+      pose proof (eval_fix _ _ _ _ _ _ _ H3 inputs outputs vars H4 H6 H8) as Hprev.
+      pose proof (eval_constraint H2 inputs outputs vars H5 H7 H9) as CtrEval.
+      exact (CtrEval :: Hprev). 
   Defined.
 
-  Definition eval{n i v i' v'}
-             (r: @r1cs n i v)(inputs: Vfp i')(vars: Vfp v')
-             {Hi: i <= i'} {Hv: v <= v'} :=
-    @eval_fix n i v i' v' r inputs vars Hi Hv.
+  Definition eval{n i o v i' o' v'}
+             (r: @r1cs n i o v)(inputs: Vfp i')(outputs: Vfp o')(vars: Vfp v')
+             {Hi: i <= i'} {Ho: o <= o'} {Hv: v <= v'} :=
+    @eval_fix n i o v i' o' v' r inputs outputs vars Hi Ho Hv.
   
-  Definition correct_lt{n i v i' v'}
-             (r: @r1cs n i v)(inputs: Vfp i')(vars: Vfp v')
-             {Hi: i <= i'}{Hv: v <= v'}: Prop :=
-    let values := @eval n i v i' v' r inputs vars Hi Hv in
+  Definition correct_lt{n i o v i' o' v'}
+             (r: @r1cs n i o v)(inputs: Vfp i')(outputs: Vfp o')(vars: Vfp v')
+             {Hi: i <= i'}{Ho: o <= o'}{Hv: v <= v'}: Prop :=
+    let values := @eval n i o v i' o' v' r inputs outputs vars Hi Ho Hv in
     Vector.Forall (fun v => v = 0:%p) values.
 
-  Definition correct{n i v}(r: @r1cs n i v)(inputs: Vfp i)(vars: Vfp v): Prop :=
-    @correct_lt n i v i v r inputs vars (Nat.le_refl i)(Nat.le_refl v).
+  Definition correct{n i o v}(r: @r1cs n i o v)(inputs: Vfp i)(outputs: Vfp o)(vars: Vfp v): Prop :=
+    @correct_lt n i o v i o v r inputs outputs vars (Nat.le_refl i)(Nat.le_refl o)(Nat.le_refl v).
              
 End R1CS.
